Engine: extended semantics of PikeVM
They now support prefix acceleration with a simulation of the .*?
prefix. This is optional, if the nextprefix is set to None, no
acceleration and no .*? is used.

Engine/PikeVM.v
@@ -105,66 +105,98 @@ Definition epsilon_step (t:thread) (c:code) (i:input): epsilon_result :=
 
 (* semantic states of the PikeVM algorithm *)
 Inductive pike_vm_state : Type :=
-| PVS (inp:input) (active: list thread) (best: option leaf) (blocked: list thread) (seen: seenpcs)
+| PVS (inp:input) (active: list thread) (best: option leaf) (blocked: list thread) (nextprefix: option nat) (seen: seenpcs)
 | PVS_final (best: option leaf).
 
+Definition pike_vm_initial_thread : thread := (0, GroupMap.empty, CanExit).
+Definition pike_vm_initial_state_lazyprefix {strs:StrSearch} (lit:literal) (inp:input) : pike_vm_state :=
+  let nextprefix := next_prefix_counter inp lit in
+  PVS inp [pike_vm_initial_thread] None [] nextprefix initial_seenpcs.
 Definition pike_vm_initial_state (inp:input) : pike_vm_state :=
-  PVS inp [(0,GroupMap.empty,CanExit)] None [] initial_seenpcs.
+  PVS inp [pike_vm_initial_thread] None [] None initial_seenpcs.
+
+Definition next_prefix_counter {strs:StrSearch} (inp: input) (lit: literal) : option nat :=
+  match advance_input inp forward with
+  | None => None
+  | Some nextinp =>
+    match input_search (prefix lit) nextinp with
+    | None => None
+    | Some nextpref => Some (idx nextpref - idx nextinp)
+    end
+  end.
 
 (* small-step semantics for the PikeVM algorithm *)
-Inductive pike_vm_step (c:code): pike_vm_state -> pike_vm_state -> Prop :=
+Inductive pike_vm_step {strs:StrSearch} (c:code) (lit:literal): pike_vm_state -> pike_vm_state -> Prop :=
 | pvs_final:
 (* moving to a final state when there are no more active or blocked threads *)
+(* FIXME: this is not exactly right with regards to the new piketree *)
   forall inp best seen,
-    pike_vm_step c (PVS inp [] best [] seen) (PVS_final best)
+    pike_vm_step c lit (PVS inp [] best [] None seen) (PVS_final best)
+| pvs_jump:
+(* if there are no more active or blocked threads and we know where the next prefix matches, *)
+(* we jump to that point *)
+  forall inp best n nextinp seen
+    (ADVANCE: advance_input_n inp (S n) forward = nextinp),
+    pike_vm_step c lit (PVS inp [] best [] (Some n) seen) (PVS nextinp [pike_vm_initial_thread] best [] (next_prefix_counter nextinp lit) initial_seenpcs)
 | pvs_end:
   (* when the list of active is empty and we've reached the end of string *)
-  forall inp best blocked seen
+  forall inp best thr blocked nextprefix seen
     (ADVANCE: advance_input inp forward = None),
-    pike_vm_step c (PVS inp [] best blocked seen) (PVS_final best)
+    pike_vm_step c lit (PVS inp [] best (thr::blocked) nextprefix seen) (PVS_final best)
 | pvs_nextchar:
   (* when the list of active threads is empty (but not blocked), restart from the blocked ones, proceeding to the next character *)
   (* reset the set of seen pcs *)
-  forall inp1 inp2 best blocked seen thr
+  forall inp1 inp2 best thr blocked seen
     (ADVANCE: advance_input inp1 forward = Some inp2),
-    pike_vm_step c (PVS inp1 [] best (thr::blocked) seen) (PVS inp2 (thr::blocked) best [] initial_seenpcs)
+    pike_vm_step c lit (PVS inp1 [] best (thr::blocked) None seen) (PVS inp2 (thr::blocked) best [] None initial_seenpcs)
+| pvs_nextchar_star:
+  forall inp1 inp2 best thr blocked seen
+    (ADVANCE: advance_input inp1 forward = Some inp2),
+    pike_vm_step c lit (PVS inp1 [] best (thr::blocked) (Some 0) seen) (PVS inp2 (thr::blocked ++ [pike_vm_initial_thread]) best [] (next_prefix_counter inp2 lit) initial_seenpcs)
+| pvs_nextchar_star_skip:
+  forall inp1 inp2 best thr blocked n seen
+    (ADVANCE: advance_input inp1 forward = Some inp2),
+    pike_vm_step c lit (PVS inp1 [] best (thr::blocked) (Some (S n)) seen) (PVS inp2 (thr::blocked) best [] (Some n) initial_seenpcs)
 | pvs_skip:
   (* when the pc has already been seen at this current index, we skip it entirely *)
-  forall inp t active best blocked seen
+  forall inp t active best blocked nextprefix seen
     (SEEN: seen_thread seen t = true),
-    pike_vm_step c (PVS inp (t::active) best blocked seen) (PVS inp active best blocked seen)
+    pike_vm_step c lit (PVS inp (t::active) best blocked nextprefix seen) (PVS inp active best blocked nextprefix seen)
 | pvs_active:
   (* generated new active threads: add them in front of the low-priority ones *)
-  forall inp t active best blocked seen nextactive
+  forall inp t active best blocked nextprefix seen nextactive
     (UNSEEN: seen_thread seen t = false)
     (STEP: epsilon_step t c inp = EpsActive nextactive),
-    pike_vm_step c (PVS inp (t::active) best blocked seen) (PVS inp (nextactive++active) best blocked (add_thread seen t))
+    pike_vm_step c lit (PVS inp (t::active) best blocked nextprefix seen) (PVS inp (nextactive++active) best blocked nextprefix (add_thread seen t))
 | pvs_match:
   (* a match is found, discard remaining low-priority active threads *)
-  forall inp t active best blocked seen
+  forall inp t active best blocked nextprefix seen
     (UNSEEN: seen_thread seen t = false)
     (STEP: epsilon_step t c inp = EpsMatch),
-    pike_vm_step c (PVS inp (t::active) best blocked seen) (PVS inp [] (Some (inp,gm_of t)) blocked (add_thread seen t))
+    pike_vm_step c lit (PVS inp (t::active) best blocked nextprefix seen) (PVS inp [] (Some (inp,gm_of t)) blocked None (add_thread seen t))
 | pvs_blocked:
   (* add the new blocked thread after the previous ones *)
-  forall inp t active best blocked seen newt
+  forall inp t active best blocked nextprefix seen newt
     (UNSEEN: seen_thread seen t = false)
     (STEP: epsilon_step t c inp = EpsBlocked newt),
-    pike_vm_step c (PVS inp (t::active) best blocked seen) (PVS inp active best (blocked ++ [newt]) (add_thread seen t)).
+    pike_vm_step c lit (PVS inp (t::active) best blocked nextprefix seen) (PVS inp active best (blocked ++ [newt]) nextprefix (add_thread seen t)).
 
 (** * PikeVM properties  *)
 
-Theorem pikevm_deterministic:
-  forall c pvso pvs1 pvs2
-    (STEP1: pike_vm_step c pvso pvs1)
-    (STEP2: pike_vm_step c pvso pvs2),
+Theorem pikevm_deterministic {strs:StrSearch}:
+  forall c lit pvso pvs1 pvs2
+    (STEP1: pike_vm_step c lit pvso pvs1)
+    (STEP2: pike_vm_step c lit pvso pvs2),
     pvs1 = pvs2.
 Proof.
-  intros c pvso pvs1 pvs2 STEP1 STEP2. inversion STEP1; subst.
+  intros c lit pvso pvs1 pvs2 STEP1 STEP2. inversion STEP1; subst.
   - inversion STEP2; subst; auto. 
-  - inversion STEP2; subst; auto. rewrite ADVANCE in ADVANCE0; inversion ADVANCE0.
+  - inversion STEP2; subst; auto.
+  - inversion STEP2; subst; auto; rewrite ADVANCE in ADVANCE0; inversion ADVANCE0.
   - inversion STEP2; subst; auto; rewrite ADVANCE in ADVANCE0; inversion ADVANCE0.
     subst. auto.
+  - inversion STEP2; subst; auto; rewrite ADVANCE in ADVANCE0; inversion ADVANCE0; auto.
+  - inversion STEP2; subst; auto; rewrite ADVANCE in ADVANCE0; inversion ADVANCE0; auto.
   - inversion STEP2; subst; auto; rewrite UNSEEN in SEEN; inversion SEEN.
   - inversion STEP2; subst; auto; try (rewrite UNSEEN in SEEN; inversion SEEN);
       rewrite STEP in STEP0; inversion STEP0.
@@ -176,17 +208,23 @@ Proof.
     subst. auto.
 Qed.
 
-Theorem pikevm_progress:
-  forall c inp active best blocked seen,
+Theorem pikevm_progress {strs:StrSearch}:
+  forall c lit inp active best blocked nextprefix seen,
   exists pvs_next,
-    pike_vm_step c (PVS inp active best blocked seen) pvs_next.
+    pike_vm_step c lit (PVS inp active best blocked nextprefix seen) pvs_next.
 Proof.
-  intros c inp active best blocked seen.
+  intros c lit inp active best blocked nextprefix seen.
   destruct active as [|[[pc gm] b] active].
   - destruct blocked as [|t blocked].
-    + eexists. econstructor.
+    + destruct nextprefix.
+      * eexists. now apply pvs_jump.
+      * eexists. apply pvs_final.
     + destruct (advance_input inp forward) eqn:INP.
-      * eexists. apply pvs_nextchar. eauto.
+      * destruct nextprefix.
+        -- destruct n.
+          ++ eexists. apply pvs_nextchar_star. eauto.
+          ++ eexists. apply pvs_nextchar_star_skip. eauto.
+        -- eexists. apply pvs_nextchar. eauto.
       * eexists. apply pvs_end. eauto.
   - destruct (seen_thread seen (pc,gm,b)) eqn:SEEN.
     { eexists. apply pvs_skip. auto. }
